Let's assume here that one player have a periodical stategy,
and that the other one has an exponential strategy.
We will denote :
$ \Gamma \left( \alpha,\:\varphi,\:\lambda \right) $
the average gain rate for the player 0 with :

\[t_{0,\:n}=n.\alpha+\varphi\qquad\text{et}\qquad
\proba{t_{1,\:n+1}\leq t_{1,n}+\delta\;|\;t_{1,\:n+1}\geq t_{1,n}}
  =\lambda.\int_0^\delta \ee{-\lambda.x}.\dd{x}\]

\manque{DÃ©monstration}

We can proove that, for $ \varphi = 0 $ we have :

\[ \Gamma \left( \alpha,\:0,\:\lambda \right) = \int_0^1x.p\left(x\right)\dd{x} \]
with $p\left(x\right) = \lambda.\ee{-\lambda.x} $